$e^{i\theta}=\cos \theta + i\sin \theta$
$e^{-i\theta}=\cos \theta-i\sin \theta$
$$
\begin{gather}
e^{i\theta}+e^{-i\theta}=2\cos \theta &  \\
e^{i\theta}-e^{-i\theta}=2i\sin \theta \\
\frac{{e^{i\theta}+e^{-i\theta}}}{2}=\cos \theta \\
\frac{{e^{i\theta}-e^{-i\theta}}}{2i}=\sin \theta
\end{gather}
$$
$a^x$ has the exponential generating sequence of $\ln(a)^n$
$$
\begin{bmatrix}
a & b \\
c & d
\end{bmatrix}
$$
$ad-bd$
Diagonal method for 3x3 cause i'm lazy

$$
\begin{gather}
U=-\mu \cdot B=-(\mu _{x}B_{x}+\mu_{y}B_{y}+\mu_{z}B_{z}) \\
F=-\nabla U= \nabla (\mu _{x}B_{x}+\mu_{y}B_{y}+\mu_{z}B_{z}) \\
F_{z}=\mu_{z}\frac{dB_{z}}{dz} \\ 
\end{gather}
$$





The commutator of two matrices/operators $[\hat{A},\hat{B}] = \hat{A}\hat{B}-\hat{B}\hat{A}$
$$
\begin{gather}
[\hat{A},\hat{B}]=-[\hat{B},\hat{A}] \\
[\hat{A},\hat{B}+\hat{C}]=[\hat{A},\hat{B}]+[\hat{A},\hat{C}] \\
[\hat{A},\hat{B}\hat{C}]=[\hat{A},\hat{B}]\hat{C}+\hat{B}[\hat{A},\hat{C}]
\end{gather}
$$
Rotations do not commute.
He proved that:
$$\begin{gather}
[\hat{J}_x,\hat{J}_y]=i\hbar \hat{J}_z \\
[\hat{J}_z,\hat{J}_x]=i\hbar \hat{J}_y \\
[\hat{J}_y,\hat{J}_z]=i\hbar \hat{J}_x
\end{gather}$$
Two matrices commute if $[\hat{A},\hat{B}]=0$ or in other words $\hat{A}\hat{B}=\hat{B}\hat{A}$

non degenerate if for each eigenvalue there is one eigenstate.
degenerate is if for at least one eigenvalue there are multiple eigenstates.

If two matrices $\hat{A},\hat{B}$ commute and are hermitian, then as long as $\hat{A}$ is non degenerate, every eigenstate of $\hat{A}$ is an eigenstate of $\hat{B}$, but not every eigenstate of $\hat{B}$ is an eigenstate of $\hat{A}$. They share the eigenstates. If you measure one eigenstate in A it implies the same eigenstate in B

Operators he introduced:
$$
\begin{gather}
\hat{J}^2=\hat{J}_{x}^2+\hat{J}_{y}^2+\hat{J}_{z}^2 \\
\hat{J}_{+}=\hat{J}_{x}+i\hat{J}_{y} \\
\hat{J}_{-}=\hat{J}_{x}-i\hat{J}_{y} \\
\hat{J}_{+}^+=\hat{J}_{-}
\end{gather}
$$

Also
$$
\begin{gather}
\hat{J}_{Z}\ket{\lambda ,m}= m\hbar\ket{\lambda ,m} \\
\hat{J}^2\ket{\lambda ,m}= m\hbar^2\ket{\lambda ,m}
\end{gather}
$$
